First draft of semantics for stack language

SourceSemantics.dfy
@@ -1,6 +1,8 @@
 
 
 include "Prelude.dfy"
+include "Common.dfy"
+include "Primitives.dfy"
 include "SourceSyntax.dfy"
 include "SourceTyping.dfy"
 
@@ -53,29 +55,6 @@ predicate method IsBool(b: bool, e: Expr) {
 predicate method IsLiteral(i: int, e: Expr) {
   if !e.Literal? then false
   else match e case Literal(l) => l == i
-}
-
-predicate method BoolOpDenotes(op: BoolOp, b1: bool, b2: bool, result: bool) {
-  match op
-    case Or  => result == b1 || b2
-    case And => result == b1 && b2
-}
-
-predicate method RelOpDenotes(op: RelOp, v1: int, v2: int, result: bool) {
-  match op
-    case Eq  => result == (v1 == v2)
-    case NEq => result == (v1 != v2)
-    case LT  => result == (v1 < v2)
-    case LTE => result == (v1 <= v2)
-}
-
-predicate method MathOpDenotes(op: MathOp, v1: int, v2: int, result: int) {
-  match op
-    case Plus      =>           result == v1 + v2
-    case Times     =>           result == v1 * v2
-    case Minus     =>           result == v1 - v2
-    case DividedBy => v2 != 0 ==> result == v1 / v2  // division by zero is undefined
-    case Mod       => v2 != 0 ==> result == v1 % v2  // division by zero is undefined
 }
 
 inductive predicate EvalExpr(d: TopLevel, s: State, e: Expr, r: Expr)
