StackSemantics.dfy
@@ -1,5 +1,124 @@
 
 include "Prelude.dfy"
 include "Common.dfy"
+include "Primitives.dfy"
 include "StackTyping.dfy"
 include "StackSubtyping.dfy"
+
+predicate method StepOperation(o: operation, s: sigma, v: value)
+{
+  match o
+    case not =>
+      |s| == 1 && s[0].boolean? &&
+      v.boolean? &&
+      s[0].getBoolean == !v.getBoolean
+    case const(x) =>
+      |s| == 0 &&
+      v == x
+    case read(t) =>
+      |s| == 0 &&
+      TypeValue(v) == t
+    case printf(format) =>
+      var types := SeqFromList(Lefts(format));
+      |s| == |types| &&
+      forall i | 0 <= i < |s| :: TypeValue(s[i]) == types[i]
+    case binary(o) =>
+      |s| == 2 &&
+      match o
+        case RelOp(o) =>
+          v.boolean? &&
+          s[0].integer? && s[1].integer? &&
+          RelOpDenotes(o, s[0].getInteger, s[1].getInteger, v.getBoolean)
+        case MathOp(o) =>
+          v.integer? &&
+          s[0].integer? && s[1].integer? &&
+          MathOpDenotes(o, s[0].getInteger, s[1].getInteger, v.getInteger)
+        case BoolOp(o) =>
+          v.boolean? &&
+          s[0].boolean? && s[1].boolean? &&
+          BoolOpDenotes(o, s[0].getBoolean, s[1].getBoolean, v.getBoolean)
+}
+
+predicate method StepCommand(c: command, s: sigma, s': sigma)
+{
+  match c
+    case store(n) =>
+      n < |s| &&
+      s' == s[n := s[0]][1..]
+    case load(n) =>
+      n < |s| &&
+      s' == [s[n]] + s
+    case pop(n) =>
+      n < |s| &&
+      s' == s[n ..]
+    case apply(n, o) =>
+      n <= |s| &&
+      var (s1, s2) := Split(n, s);
+      0 < |s'| &&
+      StepOperation(o, s1, s'[0]) &&
+      s'[1..] == s2
+}
+
+predicate method StepJump(d: delta, j: jump, phi: phi, phi': phi, b: block)
+{
+  match j
+    case halt => false
+    case goto(nu) =>
+      nu in d &&
+      |phi| == |phi'| == 0 &&
+      b == d[nu]
+    case branch(nu1, nu2) =>
+      nu1 in d && nu2 in d &&
+      |phi| == |phi'| == 1 &&
+      var nu := phi[0].0;
+      var s := phi[0].1;
+      0 < |s| &&
+      phi' == [(nu, s[1..])] &&
+      s[0].boolean? &&
+      b == d[if s[0].getBoolean then nu1 else nu2]
+    case call(n, nuJ, nuR) =>
+      nuJ in d && nuR in d &&
+      |phi| == 1 && |phi'| == 2 &&
+      var nu := phi[0].0;
+      var s := phi[0].1;
+      n <= |s| &&
+      var (s', s'') := Split(n, s);
+      phi' == [(nuR, s''), (nu, s')] &&
+      b == d[nuJ]
+    case ret(n) =>
+      |phi| == 2 && |phi'| == 1 &&
+      var nuR := phi[0].0;
+      var ss  := phi[0].1;
+      n <= |ss| &&
+      var (s_check, _) := Split(n, ss);
+      var nu := phi[1].0;
+      var s  := phi[1].1;
+      phi' == [(nu, s_check + s)] &&
+      nuR in d && b == d[nuR]
+}
+
+predicate method StepBlock(d: delta, b: block, phi: phi, phi': phi, b': block)
+{
+  var (cs, j) := b;
+  exists n, n' |
+    0 <= n < |phi| &&
+    0 <= n' < |phi'| ::
+    match cs
+      case Nil => StepJump(d, j, phi[..n], phi'[..n'], b')
+      case Cons(c, cs) =>
+        var nu := phi[0].0;
+        var s  := phi[0].1;
+        phi'[0].0 == nu &&
+        phi'[1..] == phi[1..] &&
+        var s' := phi'[0].1;
+        StepCommand(c, s, s') &&
+        b == (cs, j)
+}
+
+inductive predicate StepBlockStar(d: delta, b: block, phi: phi, phi'': phi, b'': block)
+{
+  (b == b'' && phi == phi'') ||
+    exists b', phi' ::
+      StepBlock(d, b, phi, phi', b') &&
+      StepBlockStar(d, b', phi', phi'', b'')
+}
