Primitives.dfy
@@ -1,0 +1,25 @@
+include "Prelude.dfy"
+include "Common.dfy"
+
+predicate method BoolOpDenotes(op: BoolOp, b1: bool, b2: bool, result: bool) {
+  match op
+    case Or  => result == b1 || b2
+    case And => result == b1 && b2
+}
+
+predicate method RelOpDenotes(op: RelOp, v1: int, v2: int, result: bool) {
+  match op
+    case Eq  => result == (v1 == v2)
+    case NEq => result == (v1 != v2)
+    case LT  => result == (v1 < v2)
+    case LTE => result == (v1 <= v2)
+}
+
+predicate method MathOpDenotes(op: MathOp, v1: int, v2: int, result: int) {
+  match op
+    case Plus      =>             result == v1 + v2
+    case Times     =>             result == v1 * v2
+    case Minus     =>             result == v1 - v2
+    case DividedBy => v2 != 0 ==> result == v1 / v2  // division by zero is undefined
+    case Mod       => v2 != 0 ==> result == v1 % v2  // division by zero is undefined
+}
